m

DynamoDbEncryption/dafny/DynamoDbEncryption/test/BeaconTestFixtures.dfy
@@ -8,8 +8,15 @@ module BeaconTestFixtures {
   import opened StandardLibrary
   import opened UInt = StandardLibrary.UInt
   import opened AwsCryptographyDynamoDbEncryptionTypes
+  import opened DynamoDbEncryptionUtil
   import DDB = ComAmazonawsDynamodbTypes
   import SE = AwsCryptographyStructuredEncryptionTypes
+  import KeyStore
+  import KMS = Com.Amazonaws.Kms
+  import DDBC = Com.Amazonaws.Dynamodb
+  import KTypes = AwsCryptographyKeyStoreTypes
+  import SI = SearchableEncryptionInfo
+  import Aws.Cryptography.Primitives
 
   method expect_equal<T(==)>(a: T, b: T)
     ensures a == b
@@ -92,24 +99,51 @@ module BeaconTestFixtures {
   const NameTitleBeacon := StandardBeacon(name := "NameTitleField", length := 8, loc := None)
   const NameVirtField := VirtualField(name := "NameVirtField", parts := [VPart1])
 
-  const keySource : BeaconKeySource;
+  method GetKeyStore() returns (output : SI.ValidStore)
+    ensures fresh(output.Modifies)
+  {
+    var kmsClient :- expect KMS.KMSClient();
+    var ddbClient :- expect DDBC.DynamoDBClient();
+    var keyStoreConfig := KTypes.KeyStoreConfig(
+      ddbTableName := Some("foo"),
+      ddbClient := Some(ddbClient),
+      kmsClient := Some(kmsClient)
+    );
 
-  // as empty as possible
-  const EmptyBeacons := BeaconVersion (
-    version := 1,
-    keySource := keySource,
-    standardBeacons := [std2],
-    compoundBeacons := None,
-    virtualFields := None
-  )
+    var store :- expect KeyStore.KeyStore(keyStoreConfig);
+    return store;
+  }
 
-  const LotsaBeacons := BeaconVersion (
-    version := 1,
-    keySource := keySource,
-    standardBeacons := [std2, std4, std6, NameTitleBeacon, NameB, TitleB],
-    compoundBeacons := Some([NameTitle, YearName, Mixed]),
-    virtualFields := Some([NameTitleField])
-  )
+  method GetEmptyBeacons() returns (output : BeaconVersion)
+    ensures output.keyStore.ValidState()
+    ensures fresh(output.keyStore.Modifies)
+  {
+    var store := GetKeyStore();
+    return BeaconVersion (
+      version := 1,
+      keyStore := store,
+      keySource := single(SingleKeyStore(keyId := "foo", cacheTTL := 42)),
+      standardBeacons := [std2],
+      compoundBeacons := None,
+      virtualFields := None
+    );
+  }
+
+  method GetLotsaBeacons() returns (output : BeaconVersion)
+    ensures output.keyStore.ValidState()
+    ensures fresh(output.keyStore.Modifies)
+  {
+    var store := GetKeyStore();
+    return BeaconVersion (
+      version := 1,
+      keyStore := store,
+      keySource := single(SingleKeyStore(keyId := "foo", cacheTTL := 42)),
+      standardBeacons := [std2, std4, std6, NameTitleBeacon, NameB, TitleB],
+      compoundBeacons := Some([NameTitle, YearName, Mixed]),
+      virtualFields := Some([NameTitleField])
+    );
+  }
+
   const EmptyTableConfig := DynamoDbTableEncryptionConfig (
     partitionKeyName := "foo",
     sortKeyName := None,
@@ -135,6 +169,18 @@ module BeaconTestFixtures {
       "Date" := SE.SIGN_ONLY
     ]
   );
+
+  method GetLiteralSource(key: Bytes, version : BeaconVersion) returns (output : SI.KeySource)
+    requires version.keyStore.ValidState()
+    ensures output.ValidState()
+    ensures version.keyStore == output.store
+    ensures fresh(output.client.Modifies)
+    ensures fresh(output.cache)
+  {
+    var cache := new SI.DumbCache();
+    var client :- expect Primitives.AtomicPrimitives();
+    return SI.KeySource(client, cache, version.keyStore, SI.LiteralKey([1,2,3,4,5]));
+  }
 
   const SimpleItem : DDB.AttributeMap := map[
     "std2" := Std2String,
